Syntax.v
@@ -62,7 +62,6 @@ Fixpoint pfv t tag: set nat :=
 
   | notype_tlet t1 t2 => pfv t1 tag ++  pfv t2 tag
   | tlet t1 A t2 => pfv t1 tag ++ pfv A tag ++  pfv t2 tag
-  | notype_trefl => nil
   | trefl t1 t2 => pfv t1 tag ++ pfv t2 tag
 
   | notype_tfold t' => pfv t' tag
@@ -198,7 +197,6 @@ Fixpoint psubstitute t (l: list (nat * tree)) (tag: fv_tag): tree :=
 
   | notype_tlet t1 t2 => notype_tlet (psubstitute t1 l tag) (psubstitute t2 l tag)
   | tlet t1 T t2 => tlet (psubstitute t1 l tag) (psubstitute T l tag) (psubstitute t2 l tag)
-  | notype_trefl => notype_trefl
   | trefl t1 t2 => trefl (psubstitute t1 l tag) (psubstitute t2 l tag)
 
   | notype_tfold t' => notype_tfold (psubstitute t' l tag)
@@ -302,7 +300,6 @@ Fixpoint wf t k :=
   | notype_tlet t1 t2 => wf t1 k /\ wf t2 (S k)
   | tlet t1 T t2 => wf t1 k /\ wf T k /\ wf t2 (S k)
 
-  | notype_trefl => True
   | trefl t1 t2 => wf t1 k /\ wf t2 k
 
   | tfold T t' => wf T k /\ wf t' k
@@ -391,7 +388,6 @@ Fixpoint twf t k :=
   | notype_tlet t1 t2 => twf t1 k /\ twf t2 k
   | tlet t1 T t2 => twf t1 k /\ twf T k /\ twf t2 k
 
-  | notype_trefl => True
   | trefl t1 t2 => twf t1 k /\ twf t2 k
 
   | notype_tfold t => twf t k
@@ -493,7 +489,6 @@ Fixpoint open (k: nat) (t rep: tree) :=
       notype_tlet (open k t1 rep) (open (S k) t2 rep)
   | tlet t1 T t2 =>
       tlet (open k t1 rep) (open k T rep) (open (S k) t2 rep)
-  | notype_trefl => t
   | trefl t1 t2 => trefl (open k t1 rep) (open k t2 rep)
 
   | notype_tfold t' => notype_tfold (open k t' rep)
@@ -583,7 +578,6 @@ Fixpoint close (k: nat) (t: tree) (x: nat) :=
       notype_tlet (close k t1 x) (close (S k) t2 x)
   | tlet t1 T t2 =>
       tlet (close k t1 x) (close k T x) (close (S k) t2 x)
-  | notype_trefl => t
   | trefl t1 t2 => trefl (close k t1 x) (close k t2 x)
 
   | notype_tfold t' => notype_tfold (close k t' x)
@@ -675,7 +669,6 @@ Fixpoint topen (k: nat) (t rep: tree) :=
   | tlet t1 T t2 =>
       tlet (topen k t1 rep) (topen k T rep) (topen k t2 rep)
 
-  | notype_trefl => t
   | trefl t1 t2 => trefl (topen k t1 rep) (topen k t2 rep)
 
   | notype_tfold t => notype_tfold (topen k t rep)
@@ -766,7 +759,6 @@ Fixpoint tclose (k: nat) (t: tree) (x: nat) :=
       notype_tlet (tclose k t1 x) (tclose k t2 x)
   | tlet t1 T t2 =>
       tlet (tclose k t1 x) (tclose k T x) (tclose k t2 x)
-  | notype_trefl => t
   | trefl t1 t2 => trefl (tclose k t1 x) (tclose k t2 x)
 
   | notype_tfold t => notype_tfold (tclose k t x)
