ReducibilityIteTypeRules.v
@@ -653,6 +653,6 @@ Proof.
     eauto with bwf;
     eauto using subset_same with bfv;
     eauto with berased.
-  - unshelve epose proof (H23 _ ((x, notype_trefl) :: lterms) _ _ _); tac1.
-  - unshelve epose proof (H24 _ ((x, notype_trefl) :: lterms) _ _ _); tac1.
+  - unshelve epose proof (H23 _ ((x, uu) :: lterms) _ _ _); tac1.
+  - unshelve epose proof (H24 _ ((x, uu) :: lterms) _ _ _); tac1.
 Qed.
