ReducibilitySplitIteRule.v
@@ -82,8 +82,8 @@ Proof.
     repeat step || t_listutils || t_sat_cut || t_instantiate_sat3 || t_termlist || step_inversion satisfies ||
            simp_red.
 
-    - unshelve epose proof (H24 (l1 ++ (x, notype_trefl) :: (y, notype_trefl) :: lterms) _); tac1;
+    - unshelve epose proof (H24 (l1 ++ (x, uu) :: (y, uu) :: lterms) _); tac1;
         eauto 2 using satisfies_drop.
-    - unshelve epose proof (H25 (l1 ++ (x, notype_trefl) :: (y, notype_trefl) :: lterms) _); tac1;
+    - unshelve epose proof (H25 (l1 ++ (x, uu) :: (y, uu) :: lterms) _); tac1;
         eauto 2 using satisfies_drop.
 Qed.
