ReducibilitySplitMatchRule.v
@@ -98,10 +98,10 @@ Proof.
 
   t_invert_nat_value; steps.
 
-  - unshelve epose proof (H29 (l1 ++ (x, notype_trefl) :: (y, notype_trefl) :: lterms) _);
+  - unshelve epose proof (H29 (l1 ++ (x, uu) :: (y, uu) :: lterms) _);
       repeat tac1 || step_inversion NoDup;
       eauto 2 using satisfies_drop.
-  - unshelve epose proof (H30 (l1 ++ (x, notype_trefl) :: (y, notype_trefl) :: (v,v0) :: lterms) _);
+  - unshelve epose proof (H30 (l1 ++ (x, uu) :: (y, uu) :: (v,v0) :: lterms) _);
       clear H29; clear H30; repeat tac1 || step_inversion NoDup;
       eauto 2 using satisfies_drop.
 Qed.
