StrictPositivity.v
@@ -109,5 +109,4 @@ Ltac simp_spos :=
   rewrite strictly_positive_equation_55 in * ||
   rewrite strictly_positive_equation_56 in * ||
   rewrite strictly_positive_equation_57 in * ||
-  rewrite strictly_positive_equation_58 in * ||
-  rewrite strictly_positive_equation_59.
+  rewrite strictly_positive_equation_58.
