Typing.v
@@ -1068,7 +1068,6 @@ with are_equal: tvar_list -> context -> tree -> tree -> Prop :=
     are_equal tvars gamma t1 t2 ->
     are_equal tvars gamma t2 t1
 
-(* not sound anymore when using size primitive
 | AEStep: forall tvars gamma t1 t2,
     subset (fv t1) (support gamma) ->
     subset (fv t2) (support gamma) ->
@@ -1081,7 +1080,6 @@ with are_equal: tvar_list -> context -> tree -> tree -> Prop :=
     is_context tvars gamma ->
     small_step (erase_term t1) (erase_term t2) ->
     are_equal tvars gamma t1 t2
-*)
 
 | AEPairExt: forall tvars gamma t A B,
     has_type tvars gamma t (T_prod A B) ->
